Soundness proof for big-step expression semantics

hol/symb_exec/p4_bigstepScript.sml
@@ -176,14 +176,193 @@ Definition bigstep_e_exec_def:
  (bigstep_e_exec_l scope_lists (h::t) n =
   case bigstep_e_exec scope_lists h n of
   | SOME (h', n') =>
-   (case bigstep_e_exec_l scope_lists t n' of
-    | SOME (t', n'') => SOME (h'::t', n'')
-    | NONE => NONE)
+   if is_v h'
+   then
+    (case bigstep_e_exec_l scope_lists t n' of
+     | SOME (t', n'') => SOME (h'::t', n'')
+     | NONE => NONE)
+   else SOME (h'::t, n')
   | NONE => NONE)
 Termination
 WF_REL_TAC `measure ( \ t. case t of
                            | (INL (scope_lists, e, n)) => e_size e
                            | (INR (scope_lists, e_l, n)) => e3_size e_l)` >>
+fs[e_size_def] >>
+Induct_on ‘x_e_l’ >> (
+ fs[e_size_def]
+) >>
+rpt strip_tac >>
+PairCases_on ‘h’ >>
+fs[e_size_def]
+End
+
+(* Alternative experimental version for easier proofs *)
+Definition bigstep_e_exec'_def:
+ (********************)
+ (* Variable look-up *)
+ (bigstep_e_exec' (scope_lists:scope_list) (INL (e_var x)) n =
+  case lookup_vexp scope_lists x of
+  | SOME v => SOME (INL $ e_v v, n + 1)
+  | NONE => NONE)
+  /\
+ (******************************)
+ (* Struct/header field access *)
+ (bigstep_e_exec' scope_lists (INL (e_acc e_v_struct x)) n =
+  (case bigstep_e_exec' scope_lists (INL e_v_struct) n of
+   | SOME (INL $ e_v_struct', n') =>
+    if is_v e_v_struct'
+    then
+     (case e_exec_acc (e_acc e_v_struct' x) of
+      | SOME v => SOME (INL $ v, n'+1)
+      | NONE => NONE)
+    else SOME (INL $ e_acc e_v_struct' x, n')
+   | _ => NONE))
+  /\
+ (*********************************)
+ (* Struct/header field reduction *)
+ (bigstep_e_exec' scope_lists (INL (e_struct x_e_l)) n =
+  case bigstep_e_exec' scope_lists (INR (MAP SND x_e_l)) n of
+  | SOME (INR $ e_l', n') =>
+   if (EVERY is_v e_l')
+   then
+    SOME (INL $ e_v $ v_struct (ZIP (MAP FST x_e_l, vl_of_el e_l')) , n'+1)
+   else
+    SOME (INL $ e_struct (ZIP (MAP FST x_e_l, e_l')) , n')
+  | _ => NONE)
+  /\
+ (********)
+ (* Cast *)
+ (bigstep_e_exec' scope_lists (INL (e_cast cast e)) n =
+  (case bigstep_e_exec' scope_lists (INL e) n of
+   | SOME (INL $ e', n') =>
+    if is_v e'
+    then
+     (case e_exec_cast cast e' of
+      | SOME v => SOME (INL $ e_v v, n'+1)
+      | NONE => NONE)
+    else
+     SOME (INL $ e_cast cast e', n')
+   | _ => NONE))
+  /\
+ (********************)
+ (* Unary arithmetic *)
+ (bigstep_e_exec' scope_lists (INL (e_unop unop e)) n =
+  (case bigstep_e_exec' scope_lists (INL e) n of
+   | SOME (INL $ e', n') =>
+    if is_v e'
+    then 
+     (case e_exec_unop unop e' of
+      | SOME v => SOME (INL $ e_v v, n'+1)
+      | NONE => NONE)
+    else
+     SOME (INL $ e_unop unop e', n')
+   | _ => NONE))
+  /\
+ (*********************)
+ (* Binary arithmetic *)
+ (bigstep_e_exec' scope_lists (INL (e_binop e1 binop e2)) n =
+  (case bigstep_e_exec' scope_lists (INL e1) n of
+   | SOME (INL $ e1', n') =>
+    (case e1' of
+     | (e_v v) =>
+      if is_short_circuitable binop
+      then
+       (case e_exec_short_circuit v binop e2 of
+        | SOME e' => SOME (INL $ e', n'+1)
+        | NONE => NONE)
+      else
+       (case bigstep_e_exec' scope_lists (INL e2) n' of
+        | SOME (INL $ e2', n'') =>
+         if is_v e2'
+         then
+          (case e_exec_binop e1' binop e2' of
+           | SOME v' => SOME (INL $ e_v v', n''+1)
+           | NONE => NONE)
+         else
+          SOME (INL $ e_binop e1' binop e2', n'')
+        | _ => NONE)
+     | _ =>
+      SOME (INL $ e_binop e1' binop e2, n'))
+   | _ => NONE))
+  /\
+ (*****************)
+ (* Concatenation *)
+ (bigstep_e_exec' scope_lists (INL (e_concat e1 e2)) n =
+  case bigstep_e_exec' scope_lists (INL e1) n of
+  | SOME (INL $ e1', n') =>
+   if is_v_bit e1'
+   then
+    (case bigstep_e_exec' scope_lists (INL e2) n' of
+     | SOME (INL $ e2', n'') =>
+      (if is_v_bit e2'
+       then 
+        (case e_exec_concat e1' e2' of
+         | SOME v => SOME (INL $ e_v v, n''+1)
+         | NONE => NONE)
+       else
+        SOME (INL $ e_concat e1' e2', n''))
+     | _ => NONE)
+   else
+    SOME (INL $ e_concat e1' e2, n')
+  | _ => NONE)
+  /\
+ (***********)
+ (* Slicing *)
+ (bigstep_e_exec' scope_lists (INL (e_slice e1 e2 e3)) n =
+  if (is_v_bit e2 /\ is_v_bit e3)
+  then
+   (case bigstep_e_exec' scope_lists (INL e1) n of
+    | SOME (INL $ e1', n') =>
+     if is_v_bit e1'
+     then 
+      (case e_exec_slice e1' e2 e3 of
+       | SOME v => SOME (INL $ e_v v, n'+1)
+       | NONE => NONE)
+     else
+      SOME (INL $ e_slice e1' e2 e3, n')
+    | _ => NONE)
+   else NONE)
+  /\
+ (**********************)
+ (* NESTED EXPRESSIONS *)
+ (**********************)
+(*
+ (************************)
+ (* Function/extern call *)
+ (* TODO: Needs directions... *)
+ (bigstep_e_exec' scope_lists (INL (e_call funn e_l)) n =
+  case bigstep_e_exec' scope_lists (INR e_l) n of
+  | SOME (INR $ e_l', n') =>
+   SOME (INL $ e_call funn e_l', n')
+  | _ => NONE)
+ /\
+*)
+ (**********)
+ (* Select *)
+ (bigstep_e_exec' scope_lists (INL (e_select e s_l_x_l x)) n =
+  case bigstep_e_exec' scope_lists (INL e) n of
+  | SOME (INL $ e', n') =>
+   SOME (INL $ e_select e' s_l_x_l x, n')
+  | _ => NONE)
+ /\
+ (bigstep_e_exec' scope_lists (INL e) n = SOME (INL $ e,n))
+ /\
+ (bigstep_e_exec' scope_lists (INR []) n = SOME (INR $ [],n))
+ /\
+ (bigstep_e_exec' scope_lists (INR (h::t)) n =
+  case bigstep_e_exec' scope_lists (INL h) n of
+  | SOME (INL h', n') =>
+   if is_v h'
+   then
+    (case bigstep_e_exec' scope_lists (INR t) n' of
+     | SOME (INR t', n'') => SOME (INR $ h'::t', n'')
+     | _ => NONE)
+   else SOME (INR $ h'::t, n')
+  | _ => NONE)
+Termination
+WF_REL_TAC `measure ( \ (scope_lists, t, n). case t of
+                           | (INL e) => e_size e
+                           | (INR e_l) => e3_size e_l)` >>
 fs[e_size_def] >>
 Induct_on ‘x_e_l’ >> (
  fs[e_size_def]
@@ -373,552 +552,832 @@ val induct_traverse_e_then_tac tac =
 ;
 *)
 
-Theorem bigstep_e_exec_l_incr:
-!e_l e_l' scope_lists n m.
-bigstep_e_exec_l scope_lists e_l n = SOME (e_l', m) ==>
-n <= m
+Triviality e3_e1_size:
+ !l. e3_size (MAP SND l) < e1_size l + 1
 Proof
-Induct_on ‘e_l’ >> (
-rpt disch_tac >>
- fs[bigstep_e_exec_def]
-) >>
-cheat
-(*
-(* OLD *)
-Induct_on ‘h’ >> (
- fs[bigstep_e_exec_def]
-) >| [
- rpt strip_tac >>
- Cases_on ‘bigstep_e_exec_l scope_lists e_l n’ >> (
-  fs[]
- ) >>
- PairCases_on ‘x’ >>
- fs[] >>
- res_tac >>
- decide_tac,
-
- rpt strip_tac >>
- Cases_on ‘lookup_vexp scope_lists v’ >> (
-  fs[]
- ) >>
- Cases_on ‘bigstep_e_exec_l scope_lists e_l (n + 1)’ >> (
-  fs[]
- ) >>
- PairCases_on ‘x'’ >>
- fs[] >>
- res_tac >>
- decide_tac,
-
- rpt strip_tac >>
- Cases_on ‘bigstep_e_exec_l scope_lists e_l n’ >> (
-  fs[]
- ) >>
- PairCases_on ‘x’ >>
- fs[] >>
- res_tac >>
- decide_tac,
-
- rpt strip_tac >>
- Cases_on ‘bigstep_e_exec scope_lists h n’ >> (
-  fs[]
- ) >>
- PairCases_on ‘x’ >>
- fs[] >>
- Cases_on ‘is_v x0’ >> (
-  fs[]
- ) >- (
-  Cases_on ‘e_exec_acc (e_acc x0 s)’ >> (
-   fs[]
-  ) >>
-  Cases_on ‘bigstep_e_exec_l scope_lists e_l (x1 + 1)’ >> (
-   fs[]
-  ) >>
-  PairCases_on ‘x'’ >>
-  fs[] >>
-  subgoal ‘x1 + 1 <= m’ >- (
-   cheat
-  ) >>
-  PAT_X_ASSUM “!e_l' scope_lists n m.
-          (case bigstep_e_exec scope_lists h n of
-             NONE => NONE
-           | SOME (h',n') =>
-             case bigstep_e_exec_l scope_lists e_l n' of
-               NONE => NONE
-             | SOME (t',n'') => SOME (h'::t',n'')) =
-          SOME (e_l',m) ==>
-          n <= m” (fn thm => ASSUME_TAC (Q.SPECL [‘x0::x'0’, ‘scope_lists’, ‘n’, ‘m’] thm)) >>
-  rfs[] >>
-  Cases_on ‘bigstep_e_exec_l scope_lists e_l x1’ >- (
-   (* Why can't this be NONE? *)
-   cheat
-  ) >>
- PairCases_on ‘x'’ >>
- fs[] >>
- res_tac >>
- rw[]
-
-  Cases_on ‘bigstep_e_exec_l scope_lists e_l (x1 + 1)’ >> (
-   fs[]
-  ) >>
-
-  res_tac >>
-  decide_tac
- ) >>
- res_tac >>
- decide_tac
-
-
-cheat
-
 Induct_on ‘l’ >> (
- rpt strip_tac >>
- fs[bigstep_e_exec_def]
+ fs[e_size_def]
 ) >>
- Cases_on ‘bigstep_e_exec scope_lists (SND h) n’ >> (
-  fs[]
- ) >>
- PairCases_on ‘x’ >>
- fs[] >>
- Cases_on ‘bigstep_e_exec_l scope_lists (MAP SND l) x1’ >> (
-  fs[]
- ) >>
- PairCases_on ‘x’ >>
- fs[] >>
- PAT_X_ASSUM “!e. _” (fn thm => irule thm) >>
-
- Cases_on ‘is_v x0’ >> Cases_on ‘EVERY is_v x0'’ >> (
-  fs[]
- ) >>
- qexistsl_tac [‘e_v (v_struct (ZIP (MAP FST l,vl_of_el (x0'))))’, ‘scope_lists’] >>
-*)
-QED
- 
-Theorem bigstep_e_exec_incr:
-!e e' scope_lists n m.
-bigstep_e_exec scope_lists e n = SOME (e', m) ==>
-n <= m
-Proof
-Induct_on ‘e’ >> (
- fs[bigstep_e_exec_def] >>
- rpt strip_tac
-) >| [
- Cases_on ‘lookup_vexp scope_lists v’ >>
- fs[] >>
- decide_tac,
-
- bigstep_e_exec_case'_tac >>
- Cases_on ‘is_v x0’ >> (
-  fs[]
- ) >- (
-  Cases_on ‘e_exec_acc (e_acc x0 s)’ >> (
-   fs[]
-  ) >>
-  res_tac >>
-  decide_tac
- ) >>
- res_tac >>
- decide_tac,
-
- bigstep_e_exec_case'_tac >>
- Cases_on ‘is_v x0’ >> (
-  fs[]
- ) >- (
-  Cases_on ‘e_exec_unop u x0’ >> (
-   fs[]
-  ) >>
-  res_tac >>
-  decide_tac
- ) >>
- res_tac >>
- decide_tac,
-
- bigstep_e_exec_case'_tac >>
- Cases_on ‘is_v x0’ >> (
-  fs[]
- ) >- (
-  Cases_on ‘e_exec_cast c x0’ >> (
-   fs[]
-  ) >>
-  res_tac >>
-  decide_tac
- ) >>
- res_tac >>
- decide_tac,
-
- bigstep_e_exec_case'_tac >>
- Cases_on ‘is_v x0’ >- (
-  Cases_on ‘x0’ >>
-  fs[is_v] >>
-  Cases_on ‘is_short_circuitable b’ >> (
-   fs[]
-  ) >- (
-   Cases_on ‘e_exec_short_circuit v b e'’ >> (
-    fs[]
-   ) >>
-   res_tac >>
-   decide_tac
-  ) >>
-  Cases_on ‘bigstep_e_exec scope_lists e' x1’ >> (
-   fs[]
-  ) >>
-  PairCases_on ‘x’ >>
-  fs[] >>
-  Cases_on ‘is_v x0’ >> (
-   fs[]
-  ) >- (
-   Cases_on ‘e_exec_binop (e_v v) b x0’ >> (
-    fs[]
-   ) >>
-   res_tac >>
-   decide_tac
-  ) >>
-  res_tac >>
-  decide_tac
- ) >>
- Cases_on ‘x0’ >> (
-  fs[is_v] >>
-  rw[] >>
-  res_tac >>
-  decide_tac
- ),
-
- (* Concat *)
- bigstep_e_exec_case'_tac >>
- Cases_on ‘is_v_bit x0’ >> (
-  fs[]
- ) >- (
-  Cases_on ‘bigstep_e_exec scope_lists e' x1’ >> (
-   fs[]
-  ) >>
-  PairCases_on ‘x’ >>
-  fs[] >>
-  Cases_on ‘is_v_bit x0'’ >> (
-   fs[]
-  ) >- (
-   Cases_on ‘e_exec_concat x0 x0'’ >> (
-    fs[]
-   ) >>
-   res_tac >>
-   decide_tac
-  ) >>
-  res_tac >>
-  decide_tac
- ) >>
- res_tac >>
- decide_tac,
-
- bigstep_e_exec_case'_tac >>
- Cases_on ‘is_v_bit x0’ >> (
-  fs[]
- ) >- (
-  Cases_on ‘e_exec_slice x0 e' e''’ >> (
-   fs[]
-  ) >>
-  res_tac >>
-  decide_tac
- ) >>
- res_tac >>
- decide_tac,
-
- bigstep_e_exec_case'_tac >>
- res_tac >>
- decide_tac,
-
- Cases_on ‘bigstep_e_exec_l scope_lists (MAP SND l) n’ >> (
-  fs[]
- ) >>
- PairCases_on ‘x’ >>
- fs[] >>
- Cases_on ‘EVERY is_v x0’ >> (
-  (* Need to be delicate here... *)
-  FULL_SIMP_TAC std_ss [] >>
-  fs[]
- ) >> (
-  cheat
- )
-]
+Induct_on ‘h’ >>
+gen_tac >>
+Induct_on ‘p_2’ >> (
+ fs[e_size_def]
+)
 QED
 
-Theorem bigstep_e_exec_unchanged:
-!e e' scope_lists n.
-bigstep_e_exec scope_lists e n = SOME (e', n) ==>
-e = e'
-Proof
-cheat
-QED
-
-Theorem bigstep_e_exec_l_unchanged:
-!e_l e_l' scope_lists n.
-bigstep_e_exec_l scope_lists e_l n = SOME (e_l', n) ==>
-e_l = e_l'
-Proof
-cheat
-QED
-
-Theorem bigstep_e_exec_not_eq:
-!e e' scope_lists n.
-e <> e' ==>
-bigstep_e_exec scope_lists e 0 = SOME (e',n) ==>
-n <> 0
+Theorem bigstep_e_exec'_var_REWR:
+!scope_lists var n t' m v.
+bigstep_e_exec' scope_lists (INL (e_var var)) n = SOME (t',m) <=>
+(m = n + 1 /\ ?v. SOME v =  lookup_vexp scope_lists var /\ t' = (INL $ e_v v))
 Proof
 rpt strip_tac >>
-Cases_on ‘e’ >> (
- fs[bigstep_e_exec_def]
-) >| [
- Cases_on ‘lookup_vexp scope_lists v’ >>
- fs[],
-
- bigstep_e_exec_case_tac >>
- Cases_on ‘is_v x0’ >> (
+eq_tac >> (
+ rpt strip_tac >>
+ fs[bigstep_e_exec'_def] >>
+ Cases_on ‘lookup_vexp scope_lists var’ >> (
   fs[]
- ) >- (
-  Cases_on ‘e_exec_acc (e_acc x0 s)’ >> (
-   fs[]
-  )
- ) >>
- rw[] >>
- imp_res_tac bigstep_e_exec_unchanged,
+ )
+)
+QED
 
- bigstep_e_exec_case_tac >>
- Cases_on ‘is_v x0’ >> (
+Theorem bigstep_e_exec'_var_REWR:
+!scope_lists var n t' m v.
+bigstep_e_exec' scope_lists (INL (e_var var)) n = SOME (t',m) <=>
+ (m = n + 1 /\ ?v. SOME v =  lookup_vexp scope_lists var /\ t' = (INL $ e_v v))
+Proof
+rpt strip_tac >>
+eq_tac >> (
+ rpt strip_tac >>
+ fs[bigstep_e_exec'_def] >>
+ Cases_on ‘lookup_vexp scope_lists var’ >> (
   fs[]
- ) >- (
-  Cases_on ‘e_exec_unop u x0’ >> (
-   fs[]
-  )
- ) >>
- rw[] >>
- imp_res_tac bigstep_e_exec_unchanged,
+ )
+)
+QED
 
- bigstep_e_exec_case_tac >>
- Cases_on ‘is_v x0’ >> (
-  fs[]
- ) >- (
-  Cases_on ‘e_exec_cast c x0’ >> (
-   fs[]
-  )
- ) >>
- rw[] >>
- imp_res_tac bigstep_e_exec_unchanged,
-
- bigstep_e_exec_case_tac >>
- Cases_on ‘is_v x0’ >- (
-  Cases_on ‘x0’ >>
-  fs[is_v] >>
-  Cases_on ‘is_short_circuitable b’ >> (
-   fs[]
-  ) >- (
-   Cases_on ‘e_exec_short_circuit v b e0’ >> (
-    fs[]
-   )
-  ) >>
-  Cases_on ‘bigstep_e_exec scope_lists e0 x1’ >> (
-   fs[]
-  ) >>
-  PairCases_on ‘x’ >>
-  fs[] >>
-  Cases_on ‘is_v x0’ >> (
-   fs[]
-  ) >- (
-   Cases_on ‘e_exec_binop (e_v v) b x0’ >> (
-    fs[]
-   )
-  ) >>
-  subgoal ‘x1 = 0’ >- (
-   rw[] >>
-   imp_res_tac bigstep_e_exec_incr >>
-   decide_tac
-  ) >>
-  rw[] >>
-  imp_res_tac bigstep_e_exec_unchanged >>
+Theorem bigstep_e_exec'_acc_REWR:
+!scope_lists x s n t' m.
+bigstep_e_exec' scope_lists (INL (e_acc x s)) n = SOME (t',m) <=>
+ ?n' e_v_struct.
+ bigstep_e_exec' scope_lists (INL x) n = SOME (INL e_v_struct, n') /\
+ ((is_v e_v_struct /\ ?e'. e_exec_acc (e_acc e_v_struct s) = SOME e' /\ m = n' + 1 /\
+  t' = (INL e')) \/
+ (~is_v e_v_struct /\ t' = (INL (e_acc e_v_struct s)) /\ m = n'))
+Proof
+rpt strip_tac >>
+eq_tac >> (
+ rpt strip_tac >>
+ fs[bigstep_e_exec'_def]
+) >- (
+ Cases_on ‘bigstep_e_exec' scope_lists (INL x) n’ >> (
   fs[]
  ) >>
- Cases_on ‘x0’ >>
- fs[is_v] >> (
-  rw[] >>
-  imp_res_tac bigstep_e_exec_unchanged
- ),
-
- bigstep_e_exec_case_tac >>
- Cases_on ‘is_v_bit x0’ >> (
-  fs[]
- ) >- (
-  Cases_on ‘bigstep_e_exec scope_lists e0 x1’ >> (
-   fs[]
-  ) >>
-  PairCases_on ‘x’ >>
-  fs[] >>
-  Cases_on ‘is_v_bit x0'’ >> (
-   fs[]
-  ) >- (
-   Cases_on ‘e_exec_concat x0 x0'’ >> (
-    fs[]
-   )
-  ) >>
-  subgoal ‘x1 = 0’ >- (
-   rw[] >>
-   imp_res_tac bigstep_e_exec_incr >>
-   decide_tac
-  ) >>
-  rw[] >>
-  imp_res_tac bigstep_e_exec_unchanged >>
+ PairCases_on ‘x'’ >>
+ fs[] >>
+ Cases_on ‘x'0’ >>
+ fs[] >>
+ Cases_on ‘is_v x'’ >> (
   fs[]
  ) >>
- rw[] >>
- imp_res_tac bigstep_e_exec_unchanged,
-
- bigstep_e_exec_case_tac >>
- Cases_on ‘is_v_bit x0’ >> (
+ Cases_on ‘e_exec_acc (e_acc x' s)’ >> (
   fs[]
- ) >- (
-  Cases_on ‘e_exec_slice x0 e0 e1’ >> (
-   fs[]
-  )
+ )
+)
+QED
+
+Theorem bigstep_e_exec'_unop_REWR:
+!scope_lists unop e n t' m.
+bigstep_e_exec' scope_lists (INL (e_unop unop e)) n = SOME (t',m) <=>
+ ?e' n'.
+ bigstep_e_exec' scope_lists (INL e) n = SOME (INL e', n') /\
+ ((is_v e' /\ ?v. e_exec_unop unop e' = SOME v /\ m = n' + 1 /\
+  t' = (INL $ e_v v)) \/
+ (~is_v e' /\ t' = (INL (e_unop unop e')) /\ m = n'))
+Proof
+rpt strip_tac >>
+eq_tac >> (
+ rpt strip_tac >>
+ fs[bigstep_e_exec'_def]
+) >>
+Cases_on ‘bigstep_e_exec' scope_lists (INL e) n’ >> (
+ fs[]
+) >>
+PairCases_on ‘x’ >>
+fs[] >>
+Cases_on ‘x0’ >>
+fs[] >>
+Cases_on ‘is_v x’ >> (
+ fs[]
+) >>
+Cases_on ‘e_exec_unop unop x’ >> (
+ fs[]
+)
+QED
+
+Theorem bigstep_e_exec'_cast_REWR:
+!scope_lists cast x n t' m.
+bigstep_e_exec' scope_lists (INL (e_cast cast x)) n = SOME (t',m) <=>
+ ?n' e'.
+ bigstep_e_exec' scope_lists (INL x) n = SOME (INL e', n') /\
+ ((is_v e' /\ ?v. e_exec_cast cast e' = SOME v /\ m = n' + 1 /\
+  t' = (INL $ e_v v)) \/
+ (~is_v e' /\ t' = (INL (e_cast cast e')) /\ m = n'))
+Proof
+rpt strip_tac >>
+eq_tac >> (
+ rpt strip_tac >>
+ fs[bigstep_e_exec'_def]
+) >- (
+ Cases_on ‘bigstep_e_exec' scope_lists (INL x) n’ >> (
+  fs[]
  ) >>
- rw[] >>
- imp_res_tac bigstep_e_exec_unchanged,
+ PairCases_on ‘x'’ >>
+ fs[] >>
+ Cases_on ‘x'0’ >>
+ fs[] >>
+ Cases_on ‘is_v x'’ >> (
+  fs[]
+ ) >>
+ Cases_on ‘e_exec_cast cast x'’ >> (
+  fs[]
+ )
+)
+QED
 
- bigstep_e_exec_case_tac >>
- rw[] >>
- imp_res_tac bigstep_e_exec_unchanged,
-
- Cases_on ‘bigstep_e_exec_l scope_lists (MAP SND l) 0’ >> (
+Theorem bigstep_e_exec'_binop_REWR:
+!scope_lists binop e1 e2 n t' m.
+bigstep_e_exec' scope_lists (INL (e_binop e1 binop e2)) n = SOME (t',m) <=>
+ ?e1' n'.
+ bigstep_e_exec' scope_lists (INL e1) n = SOME (INL e1', n') /\
+ ((is_v e1' /\
+  ((is_short_circuitable binop /\
+    ?v e'.
+     (e1' = e_v v /\
+      e_exec_short_circuit v binop e2 = SOME e' /\
+      t' = INL e' /\ m = n' + 1)) \/
+   (~is_short_circuitable binop /\
+    ?e2' n''.
+     bigstep_e_exec' scope_lists (INL e2) n' = SOME (INL e2', n'') /\
+     ((is_v e2' /\
+       ?v'. e_exec_binop e1' binop e2' = SOME v' /\
+        t' = (INL $ e_v v') /\ m = n'' + 1) \/
+      (~is_v e2' /\
+        t' = (INL $ e_binop e1' binop e2') /\ m = n''))))
+  ) \/
+  (~is_v e1' /\ t' = (INL (e_binop e1' binop e2)) /\ m = n'))
+Proof
+rpt strip_tac >>
+eq_tac >> (
+ rpt strip_tac >>
+ fs[bigstep_e_exec'_def]
+) >- (
+ Cases_on ‘bigstep_e_exec' scope_lists (INL e1) n’ >> (
   fs[]
  ) >>
  PairCases_on ‘x’ >>
  fs[] >>
- Cases_on ‘EVERY is_v x0’ >> (
-  (* Need to be delicate here... *)
-  FULL_SIMP_TAC std_ss []
- ) >>
+ Cases_on ‘x0’ >>
  fs[] >>
- rw[] >>
- imp_res_tac bigstep_e_exec_l_unchanged >>
- rw[] >>
- fs[p4_auxTheory.ZIP_MAP_FST_SND]
-] 
+ Cases_on ‘is_v x’ >> (
+  fs[]
+ ) >> (
+  Cases_on ‘x’ >> (
+   fs[is_v]
+  )
+ ) >>
+ Cases_on ‘is_short_circuitable binop’ >> (
+  fs[]
+ ) >- (
+  Cases_on ‘e_exec_short_circuit v binop e2’ >> (
+   fs[]
+  )
+ ) >>
+ Cases_on ‘bigstep_e_exec' scope_lists (INL e2) x1’ >> (
+  fs[]
+ ) >>
+ PairCases_on ‘x’ >>
+ fs[] >>
+ Cases_on ‘x0’ >>
+ fs[] >>
+ Cases_on ‘is_v x’ >> (
+  fs[]
+ ) >>
+ Cases_on ‘e_exec_binop (e_v v) binop x’ >> (
+  fs[]
+ )
+) >> (
+ Cases_on ‘e1'’ >> (
+  fs[is_v]
+ )
+)
 QED
 
-Theorem bigstep_e_exec_not_v_bit:
+Theorem bigstep_e_exec'_concat_REWR:
+!scope_lists e1 e2 n t' m.
+bigstep_e_exec' scope_lists (INL (e_concat e1 e2)) n = SOME (t',m) <=>
+ ?e1' n'.
+ bigstep_e_exec' scope_lists (INL e1) n = SOME (INL e1', n') /\
+ ((is_v_bit e1' /\
+  (?e2' n''.
+    bigstep_e_exec' scope_lists (INL e2) n' = SOME (INL e2', n'') /\
+    ((is_v_bit e2' /\
+      ?v. e_exec_concat e1' e2' = SOME v /\
+       t' = (INL $ e_v v) /\ m = n'' + 1) \/
+     (~is_v_bit e2' /\
+       t' = (INL $ e_concat e1' e2') /\ m = n'')))) \/
+  (~is_v_bit e1' /\ t' = (INL (e_concat e1' e2)) /\ m = n'))
+Proof
+rpt strip_tac >>
+eq_tac >> (
+ rpt strip_tac >>
+ fs[bigstep_e_exec'_def]
+) >>
+Cases_on ‘bigstep_e_exec' scope_lists (INL e1) n’ >> (
+ fs[]
+) >>
+PairCases_on ‘x’ >>
+fs[] >>
+Cases_on ‘x0’ >>
+fs[] >>
+Cases_on ‘is_v_bit x’ >> (
+ fs[]
+) >>
+Cases_on ‘bigstep_e_exec' scope_lists (INL e2) x1’ >> (
+ fs[]
+) >>
+PairCases_on ‘x'’ >>
+fs[] >>
+Cases_on ‘x'0’ >>
+fs[] >>
+Cases_on ‘is_v_bit x'’ >> (
+ fs[]
+) >>
+Cases_on ‘e_exec_concat x x'’ >> (
+ fs[]
+)
+QED
+
+Theorem bigstep_e_exec'_slice_REWR:
+!scope_lists e1 e2 e3 n t' m.
+bigstep_e_exec' scope_lists (INL (e_slice e1 e2 e3)) n = SOME (t',m) <=>
+ is_v_bit e2 /\ is_v_bit e3 /\
+ ?e1' n'.
+ bigstep_e_exec' scope_lists (INL e1) n = SOME (INL e1', n') /\
+ ((is_v_bit e1' /\
+  (?v. e_exec_slice e1' e2 e3 = SOME v /\
+   t' = (INL $ e_v v) /\ m = n' + 1)) \/
+  (~is_v_bit e1' /\ t' = (INL (e_slice e1' e2 e3)) /\ m = n'))
+Proof
+rpt strip_tac >>
+eq_tac >> (
+ rpt strip_tac >>
+ fs[bigstep_e_exec'_def]
+) >>
+Cases_on ‘bigstep_e_exec' scope_lists (INL e1) n’ >> (
+ fs[]
+) >>
+PairCases_on ‘x’ >>
+fs[] >>
+Cases_on ‘x0’ >>
+fs[] >>
+Cases_on ‘is_v_bit x’ >> (
+ fs[]
+) >>
+Cases_on ‘e_exec_slice x e2 e3’ >> (
+ fs[]
+)
+QED
+
+Theorem bigstep_e_exec'_select_REWR:
+!scope_lists e s_l_x_l x n t' m.
+bigstep_e_exec' scope_lists (INL (e_select e s_l_x_l x)) n = SOME (t',m) <=>
+ ?e' n'.
+ bigstep_e_exec' scope_lists (INL e) n = SOME (INL e', n') /\
+ t' = (INL (e_select e' s_l_x_l x)) /\ m = n'
+Proof
+rpt strip_tac >>
+eq_tac >> (
+ rpt strip_tac >>
+ fs[bigstep_e_exec'_def]
+) >>
+Cases_on ‘bigstep_e_exec' scope_lists (INL e) n’ >> (
+ fs[]
+) >>
+PairCases_on ‘x'’ >>
+fs[] >>
+Cases_on ‘x'0’ >>
+fs[]
+QED
+
+Theorem bigstep_e_exec'_struct_REWR:
+!scope_lists x_e_l n t' m.
+bigstep_e_exec' scope_lists (INL (e_struct x_e_l)) n = SOME (t',m) <=>
+ ?e_l' n'.
+ bigstep_e_exec' scope_lists (INR (MAP SND x_e_l)) n = SOME (INR e_l', n') /\
+ ((EVERY is_v e_l' /\ t' = (INL (e_v (v_struct (ZIP (MAP FST x_e_l,vl_of_el e_l'))))) /\ m = n' + 1) \/
+  (~(EVERY is_v e_l') /\ t' = (INL (e_struct (ZIP (MAP FST x_e_l,e_l')))) /\ m = n')
+ )
+Proof
+rpt strip_tac >>
+eq_tac >> (
+ rpt strip_tac >>
+ fs [bigstep_e_exec'_def]
+) >- (
+ Cases_on ‘bigstep_e_exec' scope_lists (INR (MAP SND x_e_l)) n’ >> (
+  fs[]
+ ) >>
+ PairCases_on ‘x’ >>
+ fs[] >>
+ Cases_on ‘x0’ >>
+ fs[] >>
+ Cases_on ‘EVERY is_v y’ >> (
+  FULL_SIMP_TAC bool_ss []
+ ) >> (
+  fs[]
+ )
+) >>
+subgoal ‘~EVERY is_v e_l'’ >- (
+ fs[]
+) >>
+FULL_SIMP_TAC bool_ss []
+QED
+
+val bigstep_e_exec'_ind_hyp_tac =
+ PAT_X_ASSUM “!y. _” (fn thm => ASSUME_TAC (Q.SPECL [‘(INL x)’] thm)) >>
+ fs[e_size_def] >>
+ res_tac >>
+ decide_tac
+;
+
+val bigstep_e_exec'_2_ind_hyp_tac =
+ PAT_ASSUM “!y. _” (fn thm => ASSUME_TAC (Q.SPECL [‘(INL x)’] thm)) >>
+ PAT_X_ASSUM “!y. _” (fn thm => ASSUME_TAC (Q.SPECL [‘(INL x')’] thm)) >>
+ fs[e_size_def] >>
+ res_tac >>
+ decide_tac
+;
+
+Theorem bigstep_e_exec'_incr:
+!t n scope_lists t' m.
+bigstep_e_exec' scope_lists t n = SOME (t', m) ==>
+n <= m
+Proof
+measureInduct_on ‘( \ t. case t of
+                           | (INL e) => e_size e
+                           | (INR e_l) => e3_size e_l) t’ >>
+Induct_on ‘t’ >- (
+ (* INL case *)
+ Induct_on ‘x’ >> (
+  rpt strip_tac
+ ) >| [
+  (* v *)
+  fs[bigstep_e_exec'_def],
+
+  (* var *)
+  fs[bigstep_e_exec'_var_REWR],
+
+  (* list *)
+  fs[bigstep_e_exec'_def],
+
+  (* acc *)
+  fs[bigstep_e_exec'_acc_REWR] >>
+  rpt strip_tac >> (
+   bigstep_e_exec'_ind_hyp_tac
+  ),
+
+  (* unop *)
+  fs[bigstep_e_exec'_unop_REWR] >>
+  rpt strip_tac >> (
+   bigstep_e_exec'_ind_hyp_tac
+  ),
+
+  (* cast *)
+  fs[bigstep_e_exec'_cast_REWR] >>
+  rpt strip_tac >> (
+   bigstep_e_exec'_ind_hyp_tac
+  ),
+
+  (* binop *)
+  fs[bigstep_e_exec'_binop_REWR] >>
+  rpt strip_tac >- (
+   bigstep_e_exec'_ind_hyp_tac
+  ) >- (
+   bigstep_e_exec'_2_ind_hyp_tac
+  ) >- (
+   bigstep_e_exec'_2_ind_hyp_tac
+  ) >>
+  bigstep_e_exec'_ind_hyp_tac,
+
+
+  (* concat *)
+  fs[bigstep_e_exec'_concat_REWR] >>
+  rpt strip_tac >- (
+   bigstep_e_exec'_2_ind_hyp_tac
+  ) >- (
+   bigstep_e_exec'_2_ind_hyp_tac
+  ) >>
+  bigstep_e_exec'_ind_hyp_tac,
+
+  (* slice *)
+  fs[bigstep_e_exec'_slice_REWR] >>
+  rpt strip_tac >> (
+   bigstep_e_exec'_ind_hyp_tac
+  ),
+
+  (* call *)
+  fs[bigstep_e_exec'_def],
+
+  (* select *)
+  fs[bigstep_e_exec'_select_REWR] >>
+  rpt strip_tac >>
+  bigstep_e_exec'_ind_hyp_tac,
+
+  (* struct *)
+  fs[bigstep_e_exec'_struct_REWR] >>
+  rpt strip_tac >> (
+   PAT_X_ASSUM “!y. _” (fn thm => ASSUME_TAC (Q.SPECL [‘(INR (MAP SND (l:(string # e) list)))’] thm)) >>
+   fs[e_size_def, e3_e1_size] >>
+   res_tac >>
+   decide_tac
+  ),
+
+  (* header *)
+  fs[bigstep_e_exec'_def]
+ ]
+(* INR *)
+) >>
+Induct_on ‘y’ >> (
+ rpt strip_tac >>
+ fs[bigstep_e_exec'_def]
+) >>
+Cases_on ‘bigstep_e_exec' scope_lists (INL h) n’ >> (
+ fs[]
+) >>
+PairCases_on ‘x’ >>
+fs[] >>
+Cases_on ‘x0’ >>
+fs[] >>
+Cases_on ‘bigstep_e_exec' scope_lists (INR y) x1’ >> (
+ fs[]
+) >- (
+ PAT_ASSUM “!y'. _” (fn thm => ASSUME_TAC (Q.SPECL [‘(INL h)’] thm)) >>
+ fs[e_size_def] >>
+ res_tac >>
+ decide_tac
+) >>
+PairCases_on ‘x'’ >>
+fs[] >>
+Cases_on ‘x'0’ >>
+fs[] >- (
+ PAT_ASSUM “!y'. _” (fn thm => ASSUME_TAC (Q.SPECL [‘(INL h)’] thm)) >>
+ fs[e_size_def] >>
+ res_tac >>
+ decide_tac
+) >>
+PAT_ASSUM “!y'. _” (fn thm => ASSUME_TAC (Q.SPECL [‘(INL h)’] thm)) >>
+fs[e_size_def] >>
+PAT_ASSUM “!y'. _” (fn thm => ASSUME_TAC (Q.SPECL [‘(INR y)’] thm)) >>
+fs[e_size_def] >>
+res_tac >>
+Cases_on ‘is_v x’ >> (
+ fs[]
+)
+QED
+
+val bigstep_e_exec'_unchanged_ind_hyp_tac =
+ imp_res_tac bigstep_e_exec'_incr >>
+ PAT_X_ASSUM “!y. _” (fn thm => ASSUME_TAC (Q.SPECL [‘(INL x)’] thm)) >>
+ fs[e_size_def] >>
+ res_tac >>
+ fs[]
+;
+
+val bigstep_e_exec'_unchanged_2_ind_hyp_tac =
+ imp_res_tac bigstep_e_exec'_incr >>
+ PAT_ASSUM “!y. _” (fn thm => ASSUME_TAC (Q.SPECL [‘(INL x)’] thm)) >>
+ PAT_X_ASSUM “!y. _” (fn thm => ASSUME_TAC (Q.SPECL [‘(INL x')’] thm)) >>
+ fs[e_size_def] >>
+ res_tac >>
+ fs[]
+;
+
+Theorem bigstep_e_exec'_unchanged:
+!t t' scope_lists n.
+bigstep_e_exec' scope_lists t n = SOME (t', n) ==>
+t = t'
+Proof
+measureInduct_on ‘( \ t. case t of
+                           | (INL e) => e_size e
+                           | (INR e_l) => e3_size e_l) t’ >>
+Induct_on ‘t’ >- (
+ (* INL case *)
+ Induct_on ‘x’ >> (
+  rpt strip_tac
+ ) >| [
+  (* v *)
+  fs[bigstep_e_exec'_def],
+
+  (* var *)
+  fs[bigstep_e_exec'_var_REWR],
+
+  (* list *)
+  fs[bigstep_e_exec'_def],
+
+  (* acc *)
+  fs[bigstep_e_exec'_acc_REWR] >> (
+   bigstep_e_exec'_unchanged_ind_hyp_tac
+  ),
+
+  (* unop *)
+  fs[bigstep_e_exec'_unop_REWR] >> (
+   bigstep_e_exec'_unchanged_ind_hyp_tac
+  ),
+
+  (* cast *)
+  fs[bigstep_e_exec'_cast_REWR] >> (
+   bigstep_e_exec'_unchanged_ind_hyp_tac
+  ),
+
+  (* binop *)
+  fs[bigstep_e_exec'_binop_REWR] >- (
+   bigstep_e_exec'_unchanged_ind_hyp_tac
+  ) >- (
+   bigstep_e_exec'_unchanged_2_ind_hyp_tac
+  ) >- (
+   imp_res_tac bigstep_e_exec'_incr >>
+   PAT_ASSUM “!y. _” (fn thm => ASSUME_TAC (Q.SPECL [‘(INL x)’] thm)) >>
+   PAT_X_ASSUM “!y. _” (fn thm => ASSUME_TAC (Q.SPECL [‘(INL x')’] thm)) >>
+   fs[e_size_def] >>
+   subgoal ‘n = n'’ >- (
+    decide_tac
+   ) >>
+   fs[] >>
+   res_tac >>
+   fs[]
+  ) >>
+  bigstep_e_exec'_unchanged_ind_hyp_tac,
+
+
+  (* concat *)
+  fs[bigstep_e_exec'_concat_REWR] >- (
+   bigstep_e_exec'_unchanged_2_ind_hyp_tac
+  ) >- (
+   imp_res_tac bigstep_e_exec'_incr >>
+   PAT_ASSUM “!y. _” (fn thm => ASSUME_TAC (Q.SPECL [‘(INL x)’] thm)) >>
+   PAT_X_ASSUM “!y. _” (fn thm => ASSUME_TAC (Q.SPECL [‘(INL x')’] thm)) >>
+   fs[e_size_def] >>
+   subgoal ‘n = n'’ >- (
+    decide_tac
+   ) >>
+   fs[] >>
+   res_tac >>
+   fs[]
+  ) >>
+  bigstep_e_exec'_unchanged_ind_hyp_tac,
+
+  (* slice *)
+  fs[bigstep_e_exec'_slice_REWR] >> (
+   bigstep_e_exec'_unchanged_ind_hyp_tac
+  ),
+
+  (* call *)
+  fs[bigstep_e_exec'_def],
+
+  (* select *)
+  fs[bigstep_e_exec'_select_REWR] >>
+  rpt strip_tac >>
+  bigstep_e_exec'_unchanged_ind_hyp_tac,
+
+  (* struct *)
+  fs[bigstep_e_exec'_struct_REWR] >> (
+   imp_res_tac bigstep_e_exec'_incr >>
+   PAT_X_ASSUM “!y. _” (fn thm => ASSUME_TAC (Q.SPECL [‘(INR (MAP SND (l:(string # e) list)))’] thm)) >>
+   fs[e_size_def, e3_e1_size] >>
+   res_tac >>
+   gvs[GSYM ZIP_MAP_FST_SND]
+  ),
+
+  (* header *)
+  fs[bigstep_e_exec'_def]
+ ]
+(* INR *)
+) >>
+Induct_on ‘y’ >> (
+ rpt strip_tac >>
+ fs[bigstep_e_exec'_def]
+) >>
+Cases_on ‘bigstep_e_exec' scope_lists (INL h) n’ >> (
+ fs[]
+) >>
+PairCases_on ‘x’ >>
+fs[] >>
+Cases_on ‘x0’ >>
+fs[] >>
+Cases_on ‘bigstep_e_exec' scope_lists (INR y) x1’ >> (
+ fs[]
+) >- (
+ PAT_ASSUM “!y'. _” (fn thm => ASSUME_TAC (Q.SPECL [‘(INL h)’] thm)) >>
+ gs[e_size_def] >>
+ res_tac >>
+ fs[]
+) >>
+PairCases_on ‘x'’ >>
+fs[] >>
+Cases_on ‘x'0’ >>
+fs[] >- (
+ PAT_ASSUM “!y'. _” (fn thm => ASSUME_TAC (Q.SPECL [‘(INL h)’] thm)) >>
+ gs[e_size_def] >>
+ res_tac >>
+ fs[]
+) >>
+imp_res_tac bigstep_e_exec'_incr >>
+PAT_ASSUM “!y'. _” (fn thm => ASSUME_TAC (Q.SPECL [‘(INL h)’] thm)) >>
+fs[e_size_def] >>
+PAT_ASSUM “!y'.
+          (case y' of INL e => e_size e | INR e_l => e3_size e_l) <
+          e3_size y + (e_size h + 1) ==>
+          !t' scope_lists n.
+            bigstep_e_exec' scope_lists y' n = SOME (t',n) ==> y' = t'” (fn thm => ASSUME_TAC (Q.SPECL [‘(INR y)’] thm)) >>
+
+fs[e_size_def] >>
+Cases_on ‘is_v x’ >> (
+ fs[]
+) >- (
+ gvs[] >>
+ subgoal ‘x1 = n’ >- (
+  decide_tac
+ ) >>
+ fs[] >>
+ res_tac >>
+ fs[]
+) >>
+gvs[] >>
+res_tac >>
+fs[]
+QED
+
+fun bigstep_e_exec'_not_eq_ind_hyp_tac tmq =
+ PAT_X_ASSUM “!y. _” (fn thm => ASSUME_TAC (Q.SPECL [‘(INL x)’] thm)) >>
+ fs[e_size_def] >>
+ subgoal tmq >- (
+  fs[]
+ ) >>
+ res_tac
+;
+
+Theorem bigstep_e_exec'_not_eq:
+!t t' scope_lists n.
+t <> t' ==>
+bigstep_e_exec' scope_lists t 0 = SOME (t',n) ==>
+n <> 0
+Proof
+measureInduct_on ‘( \ t. case t of
+                           | (INL e) => e_size e
+                           | (INR e_l) => e3_size e_l) t’ >>
+Induct_on ‘t’ >- (
+ (* INL case *)
+ Induct_on ‘x’ >> (
+  rpt strip_tac
+ ) >| [
+  (* v *)
+  fs[bigstep_e_exec'_def],
+
+  (* var *)
+  fs[bigstep_e_exec'_var_REWR],
+
+  (* list *)
+  fs[bigstep_e_exec'_def],
+
+  (* acc *)
+  fs[bigstep_e_exec'_acc_REWR] >>
+  bigstep_e_exec'_not_eq_ind_hyp_tac ‘INL x <> ((INL e_v_struct):(e + e list))’,
+
+  (* unop *)
+  fs[bigstep_e_exec'_unop_REWR] >>
+  bigstep_e_exec'_not_eq_ind_hyp_tac ‘INL x <> ((INL e'):(e + e list))’,
+
+  (* cast *)
+  fs[bigstep_e_exec'_cast_REWR] >>
+  bigstep_e_exec'_not_eq_ind_hyp_tac ‘INL x <> ((INL e'):(e + e list))’,
+
+  (* binop *)
+  fs[bigstep_e_exec'_binop_REWR] >- (
+   imp_res_tac bigstep_e_exec'_incr >>
+   subgoal ‘n' = 0’ >- (
+    fs[]
+   ) >>
+   fs[] >>
+   imp_res_tac bigstep_e_exec'_unchanged >>
+   fs[]
+  ) >>
+  bigstep_e_exec'_not_eq_ind_hyp_tac ‘INL x <> ((INL e1'):(e + e list))’,
+
+  (* concat *)
+  fs[bigstep_e_exec'_concat_REWR] >- (
+   imp_res_tac bigstep_e_exec'_incr >>
+   subgoal ‘n' = 0’ >- (
+    fs[]
+   ) >>
+   fs[] >>
+   imp_res_tac bigstep_e_exec'_unchanged >>
+   fs[]
+  ) >>
+  bigstep_e_exec'_not_eq_ind_hyp_tac ‘INL x <> ((INL e1'):(e + e list))’,
+
+  (* slice *)
+  fs[bigstep_e_exec'_slice_REWR] >>
+  bigstep_e_exec'_not_eq_ind_hyp_tac ‘INL x <> ((INL e1'):(e + e list))’,
+
+  (* call *)
+  fs[bigstep_e_exec'_def],
+
+  (* select *)
+  fs[bigstep_e_exec'_select_REWR] >>
+  bigstep_e_exec'_not_eq_ind_hyp_tac ‘INL x <> ((INL e'):(e + e list))’,
+
+  (* struct *)
+  fs[bigstep_e_exec'_struct_REWR] >>
+  PAT_X_ASSUM “!y. _” (fn thm => ASSUME_TAC (Q.SPECL [‘(INR (MAP SND (l:(string # e) list)))’] thm)) >>
+  fs[e_size_def, e3_e1_size] >>
+  subgoal ‘INR (MAP SND l) <> (INR (MAP SND (ZIP (MAP FST l,e_l')))):(e + e list)’ >- (
+   cheat
+  ) >>
+  res_tac >>
+  ‘e_l' = MAP SND (ZIP (MAP FST l,e_l'))’ suffices_by (
+   metis_tac[]
+  ) >>
+  imp_res_tac bigstep_e_exec'_unchanged >>
+  fs[] >>
+  subgoal ‘LENGTH (MAP FST l) = LENGTH e_l'’ >- (
+   cheat
+  ) >>
+  fs[listTheory.MAP_ZIP],
+
+  (* header *)
+  fs[bigstep_e_exec'_def]
+ ]
+) >>
+(* INR *)
+Induct_on ‘y’ >> (
+ rpt strip_tac >>
+ fs[bigstep_e_exec'_def]
+) >>
+Cases_on ‘bigstep_e_exec' scope_lists (INL h) 0’ >> (
+ fs[]
+) >>
+PairCases_on ‘x’ >>
+fs[] >>
+Cases_on ‘x0’ >>
+fs[] >>
+Cases_on ‘bigstep_e_exec' scope_lists (INR y) x1’ >> (
+ fs[]
+) >- (
+ gvs[] >>
+ PAT_ASSUM “!y'. _” (fn thm => ASSUME_TAC (Q.SPECL [‘(INL h)’] thm)) >>
+ gs[e_size_def] >>
+ res_tac
+) >>
+PairCases_on ‘x'’ >>
+fs[] >>
+Cases_on ‘x'0’ >>
+fs[] >- (
+ gvs[] >>
+ PAT_ASSUM “!y'. _” (fn thm => ASSUME_TAC (Q.SPECL [‘(INL h)’] thm)) >>
+ gs[e_size_def] >>
+ res_tac
+) >>
+imp_res_tac bigstep_e_exec'_incr >>
+PAT_ASSUM “!y'. _” (fn thm => ASSUME_TAC (Q.SPECL [‘(INL h)’] thm)) >>
+fs[e_size_def] >>
+PAT_ASSUM “!y'.
+          (case y' of INL e => e_size e | INR e_l => e3_size e_l) <
+          e3_size y + (e_size h + 1) ==>
+          !t'' scope_lists'.
+            y' <> t'' ==> bigstep_e_exec' scope_lists' y' 0 <> SOME (t'',0)” (fn thm => ASSUME_TAC (Q.SPECL [‘(INR y)’] thm)) >>
+fs[e_size_def] >>
+Cases_on ‘is_v x’ >> (
+ fs[]
+) >- (
+ gvs[] >>
+ imp_res_tac bigstep_e_exec'_unchanged >>
+ fs[]
+) >>
+gs[] >>
+imp_res_tac bigstep_e_exec'_unchanged >>
+fs[]
+QED
+
+Theorem bigstep_e_exec'_not_v_bit:
 !e e' scope_lists n.
 ~is_v_bit e ==>
 is_v_bit e' ==>
-bigstep_e_exec scope_lists e 0 = SOME (e',n) ==>
+bigstep_e_exec' scope_lists (INL e) 0 = SOME (INL e',n) ==>
 n <> 0
 Proof
-cheat
+rpt strip_tac >>
+rw[] >>
+imp_res_tac bigstep_e_exec'_unchanged >>
+Cases_on ‘e’ >> Cases_on ‘e'’ >> (
+ fs[is_v_bit]
+)
 QED
 
-Theorem bigstep_e_exec_not_v:
+Theorem bigstep_e_exec'_not_v:
 !e e' scope_lists n.
 ~is_v e ==>
 is_v e' ==>
-bigstep_e_exec scope_lists e 0 = SOME (e',n) ==>
+bigstep_e_exec' scope_lists (INL e) 0 = SOME (INL e',n) ==>
 n <> 0
 Proof
-cheat
-(* OLD
-Induct_on ‘e’ >> (
- fs[is_v]
-) >>
 rpt strip_tac >>
-Cases_on ‘e'’ >> (
-
-) >> 
-fs[is_v, bigstep_e_exec_def] >| [
- Cases_on ‘lookup_vexp scope_lists v'’ >>
- fs[],
-
- bigstep_e_exec_case_tac >>
- Cases_on ‘is_v x0’ >> (
-  fs[]
- ) >>
- Cases_on ‘e_exec_acc (e_acc x0 s)’ >> (
-  fs[]
- ),
-
- bigstep_e_exec_case_tac >>
- Cases_on ‘is_v x0’ >> (
-  fs[]
- ) >>
- Cases_on ‘e_exec_unop u x0’ >> (
-  fs[]
- ),
-
- bigstep_e_exec_case_tac >>
- Cases_on ‘is_v x0’ >> (
-  fs[]
- ) >>
- Cases_on ‘e_exec_cast c x0’ >> (
-  fs[]
- ),
-
- bigstep_e_exec_case_tac >>
- Cases_on ‘is_v x0’ >> (
-  Cases_on ‘x0’ >>
-  fs[is_v]
- ) >>
- Cases_on ‘is_short_circuitable b’ >> (
-  fs[]
- ) >- (
-  Cases_on ‘e_exec_short_circuit v' b e0’ >> (
-   fs[]
-  )
- ) >>
- Cases_on ‘bigstep_e_exec scope_lists e0 x1’ >> (
-  fs[]
- ) >>
- PairCases_on ‘x’ >>
- fs[] >>
- Cases_on ‘is_v x0’ >> (
-  Cases_on ‘x0’ >>
-  fs[is_v]
- ) >>
- Cases_on ‘e_exec_binop (e_v v') b (e_v v'')’ >> (
-  fs[]
- ),
-
- bigstep_e_exec_case_tac >>
- Cases_on ‘is_v_bit x0’ >> (
-  fs[]
- ) >>
- Cases_on ‘bigstep_e_exec scope_lists e0 x1’ >> (
-  fs[]
- ) >>
- PairCases_on ‘x’ >>
- fs[] >>
- Cases_on ‘is_v_bit x0'’ >> (
-  fs[]
- ) >>
- Cases_on ‘e_exec_concat x0 x0'’ >> (
-  fs[]
- ),
-
- bigstep_e_exec_case_tac >>
- Cases_on ‘is_v_bit x0’ >> (
-  fs[]
- ) >>
- Cases_on ‘e_exec_slice x0 e0 e1’ >> (
-  fs[]
- ),
-
- bigstep_e_exec_case_tac,
-
- Cases_on ‘bigstep_e_exec_l scope_lists (MAP SND l) 0’ >> (
-  fs[]
- ) >>
- PairCases_on ‘x’ >>
- fs[] >>
- Cases_on ‘EVERY is_v x0’ >> (
-  (* Need to be delicate here... *)
-  FULL_SIMP_TAC std_ss []
- ) >>
- fs[]
-]
-*)
+rw[] >>
+imp_res_tac bigstep_e_exec'_unchanged >>
+Cases_on ‘e’ >> Cases_on ‘e'’ >> (
+ fs[is_v]
+)
 QED
 
-
+(* TODO: Fix or remove?
 fun bigstep_e_exec_sound_single_rec_tac tmq1 tmq2 =
  Cases_on ‘is_v e’ >> (
   fs[]
@@ -950,416 +1409,512 @@ fun bigstep_e_exec_sound_single_rec_tac tmq1 tmq2 =
   fs[]
  ]
 ;
+*)
 
-
-Theorem bigstep_e_exec_v:
+Theorem bigstep_e_exec'_v:
 !v scope_list g_scope_list' n.
-bigstep_e_exec (scope_list ++ g_scope_list') (e_v v) n = SOME (e_v v, n)
+bigstep_e_exec' (scope_list ++ g_scope_list') (INL (e_v v)) n = SOME (INL $ e_v v, n)
 Proof
-cheat
+fs[bigstep_e_exec'_def]
 QED
 
-Theorem bigstep_e_exec_l_all_red:
+Theorem bigstep_e_exec'_all_red:
 !e_l scope_lists n.
 unred_mem_index e_l = NONE ==>
-bigstep_e_exec_l scope_lists e_l n = SOME (e_l,n+1)
+bigstep_e_exec' scope_lists (INR e_l) n = SOME (INR e_l,n+1)
 Proof
 cheat
 QED
 
-Theorem bigstep_e_exec_l_single_unred:
+Theorem bigstep_e_exec'_single_unred:
 !e_l e_l' e' x scope_lists n.
 unred_mem_index e_l = SOME x ==>
-bigstep_e_exec_l scope_lists e_l n = SOME (e_l',n+1) ==>
-bigstep_e_exec scope_lists (EL x e_l) n = SOME (e', n+1) /\ e_l' = LUPDATE e' x e_l
+bigstep_e_exec' scope_lists (INR e_l) n = SOME (INR e_l',n+1) ==>
+bigstep_e_exec' scope_lists (INL (EL x e_l)) n = SOME (INL e', n+1) /\ e_l' = LUPDATE e' x e_l
 Proof
 cheat
+QED
+
+Triviality unred_mem_index_NONE:
+!e_l.
+EVERY is_v e_l ==>
+unred_mem_index e_l = NONE
+Proof
+Induct >- (
+ fs[unred_mem_index_def, unred_mem_def, listTheory.INDEX_FIND_def]
+) >>
+rpt strip_tac >>
+fs[unred_mem_index_def, unred_mem_def, listTheory.INDEX_FIND_def] >>
+subgoal ‘is_const h’ >- (
+ Cases_on ‘h’ >> (
+  fs[is_v, is_const_def]
+ )
+) >>
+fs[] >>
+ Cases_on ‘INDEX_FIND 1 (\e. ~is_const e) e_l’ >> (
+  fs[]
+ ) >>
+PairCases_on ‘x’ >>
+fs[] >>
+imp_res_tac index_find_first >>
+Cases_on ‘INDEX_FIND 0 (\e. ~is_const e) e_l’ >- (
+ fs[] >>
+ fs[Q.SPECL [‘e_l’, ‘1:num’] (listTheory.INDEX_FIND_add)]
+) >>
+PairCases_on ‘x’ >>
+fs[]
 QED
 
 Theorem bigstep_e_exec_sound:
-!e scope_list g_scope_list' e' apply_table_f (ext_map:'a ext_map) func_map b_func_map pars_map tbl_map.
-bigstep_e_exec (scope_list ++ g_scope_list') e 0 = SOME (e', 1) ==>
-e_exec (apply_table_f,ext_map,func_map,b_func_map,pars_map,tbl_map)
-             g_scope_list' scope_list e = SOME (e', [])
+!t scope_list g_scope_list' t' e e_l apply_table_f (ext_map:'a ext_map) func_map b_func_map pars_map tbl_map.
+bigstep_e_exec' (scope_list ++ g_scope_list') t 0 = SOME (t', 1) ==>
+(t = (INL e) ==>
+(?e'. (t' = (INL e')) /\
+ e_exec (apply_table_f,ext_map,func_map,b_func_map,pars_map,tbl_map)
+        g_scope_list' scope_list e = SOME (e', []))) /\
+(t = INR e_l ==>
+((e_l = []) \/
+ ?i. unred_mem_index e_l = SOME i /\
+ (?e'.
+ e_exec (apply_table_f,ext_map,func_map,b_func_map,pars_map,tbl_map)
+        g_scope_list' scope_list (EL i e_l) = SOME (e', []) /\
+ t' = INR (LUPDATE e' i e_l))))
 Proof
-Induct_on ‘e’ >> (
- rpt strip_tac >>
- fs[bigstep_e_exec_def, e_exec]
-) >| [
- (* var *)
- fs[lookup_vexp_def, lookup_vexp2_def] >>
- Cases_on ‘lookup_map (scope_list ++ g_scope_list') v’ >> (
+measureInduct_on ‘( \ t. case t of
+                           | (INL e) => e_size e
+                           | (INR e_l) => e3_size e_l) t’ >>
+Induct_on ‘t’ >- (
+ (* INL case *)
+ Induct_on ‘x’ >> (
+  rpt strip_tac >>
   fs[]
- ) >>
- Cases_on ‘x’ >> (
-  fs[]
- ),
+ ) >| [
+  (* v *)
+  gvs[bigstep_e_exec'_def],
 
- (* acc *)
- (*
-  val tmq1 = ‘e_exec_acc (e_acc (e_v v) s)’
-  val tmq2 = ‘e_exec_acc (e_acc x0 s)’
- *)
- bigstep_e_exec_sound_single_rec_tac ‘e_exec_acc (e_acc (e_v v) s)’ ‘e_exec_acc (e_acc x0 s)’,
-
- (* Unop *)
- bigstep_e_exec_sound_single_rec_tac ‘e_exec_unop u (e_v v)’ ‘e_exec_unop u x0’,
-
- (* Cast *)
- bigstep_e_exec_sound_single_rec_tac ‘e_exec_cast c (e_v v)’ ‘e_exec_cast c x0’,
-
- (* Binop *)
- Cases_on ‘bigstep_e_exec (scope_list ++ g_scope_list') e 0’ >> (
-  fs[]
- ) >>
- PairCases_on ‘x’ >>
- fs[] >>
- Cases_on ‘is_v e’ >- (
-  Cases_on ‘e’ >> (
-   fs[is_v]
-  ) >>
-  subgoal ‘x0 = e_v v /\ x1 = 0’ >- (
-   fs[bigstep_e_exec_v]
-  ) >>
-  gs[] >>
-  Cases_on ‘is_short_circuitable b’ >> (
-   fs[]
-  ) >- (
-   Cases_on ‘e_exec_short_circuit v b e'’ >> (
-    fs[]
-   )
-  ) >>
-  Cases_on ‘bigstep_e_exec (scope_list ++ g_scope_list') e' 0’ >> (
+  (* var *)
+  rw[] >>
+  fs[bigstep_e_exec'_var_REWR] >>
+  fs[e_exec, lookup_vexp_def, lookup_vexp2_def] >>
+  Cases_on ‘lookup_map (scope_list ++ g_scope_list') v’ >> (
    fs[]
   ) >>
   PairCases_on ‘x’ >>
-  fs[] >>
-  Cases_on ‘is_v e'’ >> (
-   fs[]
-  ) >- (
-   (* Second operand not reduced *)
+  fs[],
+
+  (* list *)
+  gvs[bigstep_e_exec'_def],
+
+  (* acc *)
+  rw[] >>
+  fs[bigstep_e_exec'_acc_REWR] >> (
    rw[] >>
-   Cases_on ‘e'’ >> (
-    fs[is_v]
-   ) >>
-   subgoal ‘x0' = e_v v' /\ x1' = 0’ >- (
-    fs[bigstep_e_exec_v]
-   ) >>
-   fs[is_v] >>
-   Cases_on ‘e_exec_binop (e_v v) b (e_v v')’ >> (
-    fs[]
-   )
-  ) >>
-  Cases_on ‘is_v x0'’ >> (
-   fs[]
+   fs[e_exec]
   ) >- (
-   (* Contradiction on n *)
-   imp_res_tac bigstep_e_exec_not_v >>
-   Cases_on ‘e_exec_binop (e_v v) b x0'’ >> (
-    fs[]
-   )
-  ) >>
-  (* Inductive case *)
-  gs[] >>
-  res_tac >>
-  fs[] >>
-  Cases_on ‘e’ >> (
-   fs[is_v_bit, bigstep_e_exec_def]
-  )
- ) >>
- (* Second operand *)
- Cases_on ‘is_v x0’ >> (
-  fs[]
- ) >- (
-  Cases_on ‘x0’ >> (
-   fs[is_v]
-  ) >>
-  subgoal ‘x1 = 1’ >- (
-   subgoal ‘is_v $ e_v v’ >- (
-    fs[is_v]
-   ) >>
-   imp_res_tac bigstep_e_exec_not_v >>
-   Cases_on ‘bigstep_e_exec (scope_list ++ g_scope_list') e' x1’ >> (
+   Cases_on ‘is_v x’ >> (
     fs[]
    ) >- (
-    Cases_on ‘e_exec_short_circuit v b e'’ >> (
+    Cases_on ‘x’ >> (
+     fs[is_v, bigstep_e_exec'_def]
+    )
+   ) >>
+   imp_res_tac bigstep_e_exec'_unchanged >>
+   fs[]
+  ) >>
+  fs[] >>
+  PAT_X_ASSUM “!y. _” (fn thm => ASSUME_TAC (Q.SPECL [‘(INL x)’] thm)) >>
+  fs[e_size_def] >>
+  res_tac >>
+  fs[] >>
+  Cases_on ‘is_v x’ >> (
+   fs[]
+  ) >>
+  Cases_on ‘x’ >> (
+   fs[is_v, bigstep_e_exec'_def]
+  ),
+
+  (* unop *)
+  rw[] >>
+  fs[bigstep_e_exec'_unop_REWR] >> (
+   rw[] >>
+   fs[e_exec]
+  ) >- (
+   Cases_on ‘is_v x’ >> (
+    fs[]
+   ) >- (
+    Cases_on ‘x’ >> (
+     fs[is_v, bigstep_e_exec'_def]
+    )
+   ) >>
+   imp_res_tac bigstep_e_exec'_unchanged >>
+   fs[]
+  ) >>
+  fs[] >>
+  PAT_X_ASSUM “!y. _” (fn thm => ASSUME_TAC (Q.SPECL [‘(INL x)’] thm)) >>
+  fs[e_size_def] >>
+  res_tac >>
+  fs[] >>
+  Cases_on ‘is_v x’ >> (
+   fs[]
+  ) >>
+  Cases_on ‘x’ >> (
+   fs[is_v, bigstep_e_exec'_def]
+  ),
+
+  (* cast *)
+  rw[] >>
+  fs[bigstep_e_exec'_cast_REWR] >> (
+   rw[] >>
+   fs[e_exec]
+  ) >- (
+   Cases_on ‘is_v x’ >> (
+    fs[]
+   ) >- (
+    Cases_on ‘x’ >> (
+     fs[is_v, bigstep_e_exec'_def]
+    )
+   ) >>
+   imp_res_tac bigstep_e_exec'_unchanged >>
+   fs[]
+  ) >>
+  fs[] >>
+  PAT_X_ASSUM “!y. _” (fn thm => ASSUME_TAC (Q.SPECL [‘(INL x)’] thm)) >>
+  fs[e_size_def] >>
+  res_tac >>
+  fs[] >>
+  Cases_on ‘is_v x’ >> (
+   fs[]
+  ) >>
+  Cases_on ‘x’ >> (
+   fs[is_v, bigstep_e_exec'_def]
+  ),
+
+  (* binop *)
+  rw[] >>
+  fs[bigstep_e_exec'_binop_REWR] >> (
+   rw[] >>
+   fs[e_exec]
+  ) >- (
+   fs[] >>
+   imp_res_tac bigstep_e_exec'_unchanged >>
+   fs[]
+  ) >- (
+   fs[] >>
+   imp_res_tac bigstep_e_exec'_incr >>
+   fs[] >>
+   imp_res_tac bigstep_e_exec'_unchanged >>
+   fs[] >>
+   Cases_on ‘x’ >> (
+    gvs[is_v]
+   )
+  ) >- (
+   Cases_on ‘is_v x’ >> (
+    fs[]
+   ) >- (
+    Cases_on ‘x’ >> (
+     gvs[is_v]
+    ) >- (
+     Cases_on ‘is_v x'’ >> (
+      fs[]
+     ) >- (
+      Cases_on ‘x'’ >> (
+       gvs[is_v]
+      ) >>
+      fs[bigstep_e_exec'_def]
+     ) >>
+     fs[bigstep_e_exec'_def] >>
+     gvs[] >>
+     PAT_X_ASSUM “!y. _” (fn thm => ASSUME_TAC (Q.SPECL [‘(INL x')’] thm)) >>
+     fs[e_size_def] >>
+     res_tac >>
      fs[]
     )
    ) >>
-   PairCases_on ‘x’ >>
+   imp_res_tac bigstep_e_exec'_incr >>
+   subgoal ‘n' = 1’ >- (
+    CCONTR_TAC >>
+    subgoal ‘n' = 0’ >- (
+     decide_tac
+    ) >>
+    fs[] >>
+    imp_res_tac bigstep_e_exec'_unchanged >>
+    fs[]
+   ) >>
    fs[] >>
-   Cases_on ‘is_short_circuitable b’ >> (
+   PAT_X_ASSUM “!y. _” (fn thm => ASSUME_TAC (Q.SPECL [‘(INL x)’] thm)) >>
+   Cases_on ‘x’ >> (
+    gvs[is_v]
+   ) >> (
+    fs[e_size_def] >>
+    res_tac >>
+    fs[] >>
+    imp_res_tac bigstep_e_exec'_unchanged >>
+    fs[]
+   )
+  ) >- (
+   fs[] >>
+   PAT_X_ASSUM “!y. _” (fn thm => ASSUME_TAC (Q.SPECL [‘(INL x)’] thm)) >>
+   fs[e_size_def] >>
+   res_tac >>
+   fs[] >>
+   Cases_on ‘x’ >> (
+    fs[bigstep_e_exec'_def]
+   )
+  ),
+
+  (* concat *)
+  rw[] >>
+  fs[bigstep_e_exec'_concat_REWR] >> (
+   rw[] >>
+   fs[e_exec]
+  ) >- (
+   fs[] >>
+   imp_res_tac bigstep_e_exec'_incr >>
+   fs[] >>
+   imp_res_tac bigstep_e_exec'_unchanged >>
+   fs[]
+  ) >- (
+   Cases_on ‘is_v_bit x’ >> (
     fs[]
    ) >- (
-    Cases_on ‘e_exec_short_circuit v b e'’ >> (
+    Cases_on ‘x’ >> (
+     gvs[is_v_bit]
+    ) >>
+    Cases_on ‘v’ >> (
+     gvs[is_v_bit]
+    ) >>
+    Cases_on ‘is_v_bit x'’ >> (
      fs[]
+    ) >- (
+     Cases_on ‘x'’ >> (
+      gvs[is_v_bit]
+     ) >>
+     fs[bigstep_e_exec'_def]
+    ) >>
+    subgoal ‘n' = 0’ >- (
+     fs[bigstep_e_exec'_def]
+    ) >>
+    fs[] >>
+    PAT_X_ASSUM “!y. _” (fn thm => ASSUME_TAC (Q.SPECL [‘(INL x')’] thm)) >>
+    fs[e_size_def] >>
+    res_tac >>
+    fs[] >>
+    imp_res_tac bigstep_e_exec'_unchanged >>
+    fs[]
+   ) >>
+   imp_res_tac bigstep_e_exec'_incr >>
+   subgoal ‘n' = 1’ >- (
+    CCONTR_TAC >>
+    subgoal ‘n' = 0’ >- (
+     decide_tac
+    ) >>
+    fs[] >>
+    imp_res_tac bigstep_e_exec'_unchanged >>
+    fs[]
+   ) >>
+   fs[] >>
+   PAT_X_ASSUM “!y. _” (fn thm => ASSUME_TAC (Q.SPECL [‘(INL x)’] thm)) >>
+   fs[e_size_def] >>
+   res_tac >>
+   fs[] >>
+   imp_res_tac bigstep_e_exec'_unchanged >>
+   fs[]
+  ) >- (
+   fs[] >>
+   PAT_X_ASSUM “!y. _” (fn thm => ASSUME_TAC (Q.SPECL [‘(INL x)’] thm)) >>
+   fs[e_size_def] >>
+   res_tac >>
+   fs[] >>
+   Cases_on ‘is_v_bit x’ >> (
+    fs[]
+   ) >>
+   Cases_on ‘x’ >> (
+    gvs[is_v_bit]
+   ) >>
+   fs[bigstep_e_exec'_def]
+  ),
+
+  (* slice *)
+  rw[] >>
+  fs[bigstep_e_exec'_slice_REWR] >> (
+   rw[] >>
+   fs[e_exec]
+  ) >- (
+   Cases_on ‘is_v_bit x’ >> (
+    fs[]
+   ) >- (
+    Cases_on ‘x’ >> (
+     fs[is_v_bit, bigstep_e_exec'_def]
     )
    ) >>
-   Cases_on ‘is_v x0’ >> (
-    fs[]
-   ) >- (
-    Cases_on ‘e_exec_binop (e_v v) b x0’ >> (
-     fs[]
-    ) >>
-    imp_res_tac bigstep_e_exec_incr >>
-    decide_tac
-   ) >>
-   imp_res_tac bigstep_e_exec_incr >>
-   decide_tac
+   imp_res_tac bigstep_e_exec'_unchanged >>
+   fs[]
   ) >>
   fs[] >>
-  Cases_on ‘bigstep_e_exec (scope_list ++ g_scope_list') e' 1’ >> (
-   fs[]
-  ) >- (
-   Cases_on ‘e_exec_short_circuit v b e'’ >> (
-    fs[]
-   )
-  ) >>
-  Cases_on ‘is_short_circuitable b’ >> (
-   fs[]
-  ) >- (
-   Cases_on ‘e_exec_short_circuit v b e'’ >> (
-    fs[]
-   )
-  ) >>
-  PairCases_on ‘x’ >>
-  fs[] >>
-  subgoal ‘~is_v x0’ >- (
-   CCONTR_TAC >>
-   fs[] >>
-   Cases_on ‘e_exec_binop (e_v v) b x0’ >> (
-    fs[]
-   ) >>
-   imp_res_tac bigstep_e_exec_incr >>
-   decide_tac
-  ) >>
-  gs[] >>
+  PAT_X_ASSUM “!y. _” (fn thm => ASSUME_TAC (Q.SPECL [‘(INL x)’] thm)) >>
+  fs[e_size_def] >>
   res_tac >>
   fs[] >>
-  subgoal ‘e' = x0’ >- (
-   imp_res_tac bigstep_e_exec_unchanged
+  Cases_on ‘is_v_bit x’ >> (
+   fs[]
   ) >>
-  Cases_on ‘e’ >> (
-   fs[is_v, bigstep_e_exec_def]
-  )
- ) >>
- Cases_on ‘x0’ >> Cases_on ‘e’ >> (
-  fs[is_v, bigstep_e_exec_def] >>
-  gs[] >>
-  res_tac >>
-  fs[]
- ),
+  Cases_on ‘x’ >> (
+   fs[is_v_bit, bigstep_e_exec'_def]
+  ),
 
- (* Concat *)
- Cases_on ‘bigstep_e_exec (scope_list ++ g_scope_list') e 0’ >> (
-  fs[]
- ) >>
- PairCases_on ‘x’ >>
- fs[] >>
- Cases_on ‘is_v_bit e’ >> (
-  fs[]
- ) >- (
-  Cases_on ‘e’ >> (
-   fs[is_v_bit]
-  ) >>
-  (* First operand not reduced *)
-  subgoal ‘x0 = e_v v /\ x1 = 0’ >- (
-   fs[bigstep_e_exec_v]
-  ) >>
-  fs[] >>
-  Cases_on ‘bigstep_e_exec (scope_list ++ g_scope_list') e' 0’ >> (
-   fs[]
-  ) >>
-  PairCases_on ‘x’ >>
-  fs[] >>
-  Cases_on ‘is_v_bit e'’ >> (
-   fs[]
-  ) >- (
-   (* Second operand not reduced *)
+  (* call *) 
+  gvs[bigstep_e_exec'_def],
+
+  (* select *)
+  rw[] >>
+  fs[bigstep_e_exec'_select_REWR] >> (
    rw[] >>
-   Cases_on ‘e'’ >> (
-    fs[is_v_bit]
-   ) >>
-   subgoal ‘x0' = e_v v' /\ x1' = 0’ >- (
-    fs[bigstep_e_exec_v]
-   ) >>
-   fs[] >>
-   Cases_on ‘v’ >> (
-    gvs[is_v_bit]
-   ) >>
-   Cases_on ‘v'’ >> (
-    gvs[is_v_bit]
-   ) >>
-   Cases_on ‘e_exec_concat (e_v (v_bit p)) (e_v (v_bit p'))’ >> (
-    fs[]
-   )
+   fs[e_exec]
   ) >>
-  (* Second operand was reduced, or e subtype contradiction *)
-  Cases_on ‘is_v_bit x0'’ >> (
+  Cases_on ‘is_v x’ >> (
    fs[]
   ) >- (
-   (* Contradiction on n *)
-   Cases_on ‘x0'’ >> (
-    fs[is_v_bit]
-   ) >>
-   imp_res_tac bigstep_e_exec_not_v_bit >>
-   Cases_on ‘e_exec_concat (e_v v) (e_v v')’ >> (
-    fs[]
+   Cases_on ‘x’ >> (
+    fs[is_v, bigstep_e_exec'_def]
    )
   ) >>
-  (* Inductive case *)
-  gs[] >>
+  PAT_X_ASSUM “!y. _” (fn thm => ASSUME_TAC (Q.SPECL [‘(INL x)’] thm)) >>
+  fs[e_size_def] >>
   res_tac >>
-  fs[] >>
-  Cases_on ‘e’ >> (
-   fs[is_v_bit, bigstep_e_exec_def]
-  )
- ) >>
- (* First operand was reduced *)
- Cases_on ‘is_v_bit x0’ >> (
-  fs[]
- ) >- (
-  subgoal ‘x1 = 1’ >- (
-   imp_res_tac bigstep_e_exec_not_v_bit >>
-   Cases_on ‘bigstep_e_exec (scope_list ++ g_scope_list') e' x1’ >> (
-    fs[]
-   ) >>
-   PairCases_on ‘x’ >>
+  fs[],
+
+  (* struct *)
+  rw[] >>
+  fs[bigstep_e_exec'_struct_REWR] >> (
+   rw[] >>
+   fs[e_exec]
+  ) >- (
    fs[] >>
-   Cases_on ‘is_v_bit x0'’ >> (
+   imp_res_tac bigstep_e_exec'_unchanged >>
+   fs[] >>
+   Cases_on ‘unred_mem_index e_l'’ >> (
     fs[]
-   ) >- (
-    Cases_on ‘e_exec_concat x0 x0'’ >> (
-     fs[]
-    ) >>
-    imp_res_tac bigstep_e_exec_incr >>
-    decide_tac
    ) >>
-   imp_res_tac bigstep_e_exec_incr >>
-   decide_tac
-  ) >>
-  fs[] >>
-  Cases_on ‘bigstep_e_exec (scope_list ++ g_scope_list') e' 1’ >> (
+   (* Contradiction on unreduced element in e_l' *)
+   imp_res_tac unred_mem_index_NONE >>
    fs[]
   ) >>
-  PairCases_on ‘x’ >>
   fs[] >>
-  subgoal ‘~is_v_bit x0'’ >- (
-   CCONTR_TAC >>
-   fs[] >>
-   Cases_on ‘e_exec_concat x0 x0'’ >> (
-    fs[]
-   ) >>
-   imp_res_tac bigstep_e_exec_incr >>
-   decide_tac
-  ) >>
-  fs[] >>
-  gs[] >>
+  PAT_X_ASSUM “!y. _” (fn thm => ASSUME_TAC (Q.SPECL [‘(INR (MAP SND (l:(string # e) list)))’] thm)) >>
+  fs[e_size_def, e3_e1_size] >>
   res_tac >>
-  fs[] >>
-  subgoal ‘e' = x0'’ >- (
-   imp_res_tac bigstep_e_exec_unchanged
+  Cases_on ‘l’ >- (
+   fs[bigstep_e_exec'_def, e_exec]
   ) >>
-  fs[]
- ) >>
- (* Inductive case *)
- gs[] >>
- res_tac >>
- fs[] >>
- Cases_on ‘e’ >> (
-  fs[is_v_bit, bigstep_e_exec_def]
- ),
-
- (* Slice *)
- Cases_on ‘bigstep_e_exec (scope_list ++ g_scope_list') e 0’ >> (
-  fs[]
- ) >>
- PairCases_on ‘x’ >>
- fs[] >>
- Cases_on ‘is_v_bit e’ >> (
-  fs[]
- ) >- (
-  Cases_on ‘e’ >> (
-   fs[is_v_bit]
-  ) >>
-  subgoal ‘x0 = e_v v /\ x1 = 0’ >- (
-   fs[bigstep_e_exec_v]
-  ) >>
-  fs[] >>
-  Cases_on ‘e_exec_slice (e_v v) e' e''’ >> (
-   fs[]
-  )
- ) >>
- subgoal ‘~is_v_bit x0’ >> (
-  CCONTR_TAC >>
-  fs[] >>
-  Cases_on ‘e_exec_slice x0 e' e''’ >> (
+  fs[e_exec] >>
+  Cases_on ‘unred_mem_index (SND h::MAP SND t)’ >> (
    fs[]
   ) >>
-  rfs[] >>
-  imp_res_tac bigstep_e_exec_unchanged >>
-  fs[is_v_bit]
- ) >>
- gs[] >>
- res_tac >>
- fs[],
+  PAT_X_ASSUM “!tbl_map pars_map func_map ext_map b_func_map apply_table_f. _” (fn thm => ASSUME_TAC (Q.SPECL [‘tbl_map’, ‘pars_map’, ‘func_map’, ‘ext_map’, ‘b_func_map’, ‘apply_table_f’] thm)) >>
+  fs[],
 
- (* Select *)
- Cases_on ‘bigstep_e_exec (scope_list ++ g_scope_list') e 0’ >> (
-  fs[]
- ) >>
- PairCases_on ‘x’ >>
- fs[] >>
- Cases_on ‘is_v e’ >> (
-  fs[]
- ) >- (
-  Cases_on ‘e’ >> (
-   fs[is_v]
-  ) >>
-  fs[bigstep_e_exec_v]
- ) >>
- gs[] >>
- res_tac >>
- fs[],
-
- (* Struct entry *)
-(* OLD
- Induct_on ‘l’ >> (
-  fs[bigstep_e_exec_def]
- ) >- (
-  fs[unred_mem_index_def, unred_mem_def, listTheory.INDEX_FIND_def]
- ) >>
-*)
+  (* header *)
+  gvs[bigstep_e_exec'_def]
+ ]
+) >>
+(* INR *)
+Induct_on ‘y’ >> (
  rpt strip_tac >>
- Cases_on ‘unred_mem_index (MAP SND l)’ >> (
-  fs[]
- ) >- (
-  imp_res_tac bigstep_e_exec_l_all_red >>
-  Cases_on ‘bigstep_e_exec_l (scope_list ++ g_scope_list') (MAP SND l) 0’ >> (
-   fs[]
-  ) >>
-  PairCases_on ‘x’ >>
-  fs[] >>
-  subgoal ‘EVERY is_v x0’ >- (
-   cheat
-  ) >>
-  fs[] >>
-  gvs[]
- ) >>
- Cases_on ‘bigstep_e_exec_l (scope_list ++ g_scope_list') (MAP SND l) 0’ >> (
+ fs[bigstep_e_exec'_def]
+) >>
+Cases_on ‘bigstep_e_exec' (scope_list ++ g_scope_list') (INL h) 0’ >> (
+ fs[]
+) >>
+PairCases_on ‘x’ >>
+fs[] >>
+Cases_on ‘x0’ >>
+fs[] >>
+Cases_on ‘is_v x’ >> (
+ fs[]
+) >- (
+ (* Same as with old definition *)
+ Cases_on ‘bigstep_e_exec' (scope_list ++ g_scope_list') (INR y) x1’ >> (
   fs[]
  ) >>
  PairCases_on ‘x'’ >>
  fs[] >>
- subgoal ‘~EVERY is_v x'0’ >- (
-  cheat
+ Cases_on ‘x'0’ >>
+ fs[] >>
+ subgoal ‘x1 = 0 \/ x1 = 1’ >- (
+  imp_res_tac bigstep_e_exec'_incr >>
+  decide_tac
+ ) >- (
+  (* x1 = 0: y reduction contributes the step *)
+  gs[] >>
+  imp_res_tac bigstep_e_exec'_unchanged >>
+  gs[] >>
+  PAT_ASSUM “!y'. _” (fn thm => ASSUME_TAC (Q.SPECL [‘(INR y)’] thm)) >>
+  fs[e_size_def] >>
+  subgoal ‘e3_size y < e3_size e_l’ >- (
+   gvs[e_size_def]
+  ) >>
+  fs[] >>
+  res_tac >>
+  PAT_X_ASSUM “!tbl_map pars_map func_map ext_map b_func_map apply_table_f. _” (fn thm => ASSUME_TAC (Q.SPECL [‘tbl_map’, ‘pars_map’, ‘func_map’, ‘ext_map’, ‘b_func_map’, ‘apply_table_f’] thm)) >>
+  fs[] >>
+  gvs[] >- (
+   fs[bigstep_e_exec'_def]
+  ) >>
+  fs[] >>
+  qexists_tac ‘i+1’ >>
+  gvs[] >>
+  rpt strip_tac >- (
+   (* Not true? h could be any expression that is not reduced further.. *)
+   subgoal ‘is_const h’ >- (
+    Cases_on ‘h’ >> (
+     fs[is_v, is_const_def]
+    )
+   ) >>
+   fs[unred_mem_index_def, unred_mem_def, listTheory.INDEX_FIND_def] >>
+   fs[Q.SPECL [‘y’, ‘1:num’] (listTheory.INDEX_FIND_add)] >>
+   Cases_on ‘INDEX_FIND 0 (\e. ~is_const e) y’ >> (
+    fs[]
+   ) >>
+   PairCases_on ‘x’ >>
+   fs[]
+  ) >>
+  qexists_tac ‘e'’ >>
+  subgoal ‘(EL (i + 1) (h::y)) = (EL i y)’ >- (
+   fs[GSYM p4_auxTheory.SUC_ADD_ONE, listTheory.EL_restricted]
+  ) >>
+  fs[GSYM p4_auxTheory.SUC_ADD_ONE, listTheory.LUPDATE_def]
  ) >>
- FULL_SIMP_TAC std_ss [] >>
- rw[] >>
- imp_res_tac bigstep_e_exec_l_single_unred >>
- (* TODO: This requires some further thought... *)
- cheat
-]
+ (* x1 = 1: h reduction contributes the step *)
+ gvs[] >>
+ subgoal ‘~is_const h’ >- (
+  CCONTR_TAC >>
+  Cases_on ‘h’ >> (
+   fs[is_const_def, bigstep_e_exec'_def]
+  )
+ ) >>
+ PAT_ASSUM “!y'. _” (fn thm => ASSUME_TAC (Q.SPECL [‘(INL h)’] thm)) >>
+ fs[e_size_def] >>
+ res_tac >>
+ fs[] >>
+ qexists_tac ‘0’ >>
+ fs[unred_mem_index_def, unred_mem_def, listTheory.INDEX_FIND_def, listTheory.LUPDATE_def] >>
+ imp_res_tac bigstep_e_exec'_unchanged >>
+ fs[]
+) >>
+(* New case *)
+gvs[] >>
+qexists_tac ‘0’ >>
+subgoal ‘~is_const h’ >- (
+ CCONTR_TAC >>
+ Cases_on ‘h’ >> (
+  fs[is_const_def, bigstep_e_exec'_def]
+ )
+) >>
+fs[unred_mem_index_def, unred_mem_def, listTheory.INDEX_FIND_def, listTheory.LUPDATE_def] >>
+PAT_ASSUM “!y'. _” (fn thm => ASSUME_TAC (Q.SPECL [‘(INL h)’] thm)) >>
+fs[e_size_def] >>
+res_tac >>
+fs[]
 QED
 
 Theorem scope_lists_separate:
